feat: solution for 4

proj1/src/Ex4.dfy
@@ -4,6 +4,7 @@ module Ex4 {
   import Ex3=Ex3
 
   class Set {
+    // without duplicates
     var list : Ex3.Node?
 
     ghost var footprint : set<Ex3.Node>
@@ -20,7 +21,8 @@ module Ex4 {
         else 
           footprint == list.footprint
           &&
-          content == list.content
+          content == seq2set(list.content)
+          // content == list.content
           &&
           list.Valid()
     }
@@ -33,30 +35,209 @@ module Ex4 {
       content := {};      
     }
 
-
+    /**
+      Checks if the current set contains the value v 
+     */
     method mem (v : nat) returns (b : bool)
+      requires this.Valid()
+      ensures b == (v in this.content)
     {
-   
+      if this.list == null {
+        b := false;
+        return;
+      } else {
+        b := this.list.mem(v);
+
+        // to understand that the mem check extends to this content
+        seq2seqEquiv(this.list.content, this.content, v);
+        return;
+      }
     }
 
-
+    /**
+      Adds v to the current set 
+     */
     method add (v : nat) 
+      requires this.Valid()
+      modifies this
+
+      ensures this.Valid()
+      ensures this.content == old(this.content) + {v}
     {
+      var b := this.mem(v);
+      if !b {
+        if this.list == null {
+          this.list := new Ex3.Node(v);
+          this.footprint := {this.list};
+          this.content := {v};
+        } else {
+          this.list := this.list.add(v);
+          this.footprint := this.list.footprint;
+          this.content := {v} + this.content;
+        }
+      }
     }
 
-
+    /**
+      Computes the union of the current set and the set s given as input 
+     */
     method union(s : Set) returns (r : Set)
+      requires s.Valid()
+      requires this.Valid()
+
+      ensures r.Valid()
+      ensures r.content == s.content + this.content
     {
-    
+      r := new Set();
+
+      // O(|s|)
+      if s.list != null {
+        r.list := s.list.copy();
+        r.footprint := r.list.footprint;
+        r.content := seq2set(r.list.content);
+      }
+
+      assert r.content == s.content;
+
+      // O(|s| * |this|)
+      var cur := this.list;
+
+      ghost var seen : seq<nat> := [];
+      while cur != null
+        invariant cur != null ==> cur.Valid()
+        invariant r.Valid()
+        invariant cur != null ==> this.list.content == seen + cur.content
+        invariant cur == null ==> this.content == seq2set(seen)
+        invariant r.content == s.content + seq2set(seen)
+
+        decreases if cur != null then cur.footprint else {}
+      {
+        ghost var oldR := r.content;
+        r.add(cur.val);
+        assert r.content == oldR + {cur.val};
+
+        ghost var oldSeen := seen;
+        seen := seen + [cur.val];
+        seq2seqEquiv(seen, seq2set(seen), cur.val);
+        seq2setAdd(oldSeen, cur.val);
+
+        cur := cur.next;
+      }
+
     }
 
+    method inter(s : Set) returns (r : Set)
+      requires s.Valid() 
+      requires this.Valid() 
 
-  method inter(s : Set) returns (r : Set)
+      ensures r.Valid()
+      ensures r.content == s.content * this.content
     {
-      
+      r := new Set();
+
+      // O(|s| * |this|)
+      var cur := this.list;
+      ghost var seen : seq<nat> := [];
+      while cur != null
+        invariant cur != null ==> cur.Valid()
+        invariant r.Valid()
+        invariant cur != null ==> this.list.content == seen + cur.content
+        invariant cur == null ==> this.content == seq2set(seen)
+        invariant r.content == s.content * seq2set(seen)
+        decreases if cur != null then cur.footprint else {}
+      {
+        var inIntersection := s.mem(cur.val);
+        if inIntersection {
+          ghost var oldR := r.content;
+          r.add(cur.val);
+          assert r.content == oldR + {cur.val};
+          // assert cur.val in s.content * this.content;
+        }
+
+        ghost var oldSeen := seen;
+        seen := seen + [cur.val];
+        seq2seqEquiv(seen, seq2set(seen), cur.val);
+        seq2setAdd(oldSeen, cur.val);
+
+        cur := cur.next;
+      }
 
     }
   }
 
-}
+  lemma seq2setAdd(s: seq<nat>, k: nat)
+  ensures seq2set(s + [k]) == seq2set(s) + {k}
+  {
+    if s == [] {
+    } else {
+      calc {
+            seq2set(s + [k]);
+          == { assert s == [s[0]] + s[1..]; }
+            seq2set(([s[0]] + s[1..]) + [k]);
+          == { assert ([s[0]] + s[1..]) + [k] == [s[0]] + (s[1..] + [k]);}
+            seq2set([s[0]] + (s[1..] + [k]));
+          ==
+            seq2set(s) + {k};
+      }
+    }
+  }
 
+  lemma seq2seqEquiv(s: seq<nat>, c: set<nat>, k: nat)
+    requires c == seq2set(s)
+
+    ensures k in c <==> k in s
+  {
+    if k in c {
+      seq2seqEquivAux(s, c, k);
+      assert k in s;
+
+    } else {
+      if k in s {
+          // contradiction
+          seq2seqEquivAux2(s, c, k);
+          assert k in c;
+      } else {
+
+      }
+    }
+  }
+
+  lemma seq2seqEquivAux(s: seq<nat>, c: set<nat>, k: nat)
+    requires c == seq2set(s)
+    requires k in c
+    
+    ensures k in s
+  {
+    if s == [] {
+    } else {
+      if k == s[0] {
+      } else {
+        seq2seqEquivAux(s[1..], seq2set(s[1..]), k);
+      }
+    }
+
+  }
+
+  lemma seq2seqEquivAux2(s: seq<nat>, c: set<nat>, k: nat)
+    requires c == seq2set(s)
+    requires k in s
+    
+    ensures k in c
+  {
+    if s[0] == k {
+    } else {
+      seq2seqEquivAux2(s[1..], seq2set(s[1..]), k);
+    }
+  }
+
+  lemma seq2setGood(s1: seq<nat>, s2: seq<nat>)
+    requires s1 == s2
+    ensures seq2set(s1) == seq2set(s2)
+  {
+  }
+
+  function seq2set(s: seq<nat>): set<nat>
+  {
+    if s == [] then {} else {s[0]} + seq2set(s[1..])
+  }
+}
